Update proofs

correctness/RegexCorrectness/VM/Correspondence/Refinement/Refinement.lean
@@ -1,6 +1,6 @@
 import RegexCorrectness.VM.Search
 import RegexCorrectness.VM.Correspondence.Materialize
-import RegexCorrectness.VM.Correspondence.Refinement.Simp
+-- import RegexCorrectness.VM.Correspondence.Refinement.Simp
 
 set_option autoImplicit false
 
@@ -19,14 +19,14 @@ namespace Regex.VM
 
 variable {nfa : NFA} {wf : nfa.WellFormed} {bufferSize : Nat} {it : Iterator}
   {matched : Option (Buffer bufferSize)} {matched' : Option (List (Nat × Pos))}
-  {next : SearchState nfa bufferSize} {next' : SearchState' nfa}
-  {stack : εStack nfa bufferSize} {stack' : εStack' nfa}
+  {next : SearchState (BufferStrategy bufferSize) nfa} {next' : SearchState HistoryStrategy nfa}
+  {stack : εStack (BufferStrategy bufferSize) nfa} {stack' : εStack HistoryStrategy nfa}
 
 def refineUpdate (update : List (Nat × Pos)) (buffer : Buffer bufferSize) : Prop :=
   materializeUpdates bufferSize update = buffer
 
 @[simp]
-theorem refineUpdate.empty : @refineUpdate bufferSize [] Buffer.empty := rfl
+theorem refineUpdate.empty {bufferSize : Nat} : refineUpdate HistoryStrategy.empty (BufferStrategy bufferSize).empty := rfl
 
 def refineUpdateOpt : Option (List (Nat × Pos)) → Option (Buffer bufferSize) → Prop
   | .none, .none => True
@@ -58,23 +58,23 @@ theorem refineUpdateOpt.orElse {update₁ update₂ : Option (List (Nat × Pos))
 def refineUpdates (updates : Vector (List (Nat × Pos)) nfa.nodes.size) (buffers : Vector (Buffer bufferSize) nfa.nodes.size) : Prop :=
   ∀ (i : Fin nfa.nodes.size), refineUpdate updates[i] buffers[i]
 
-def SearchState'.refines (state' : SearchState' nfa) (state : SearchState nfa bufferSize) : Prop :=
+def SearchState.refines (state' : SearchState HistoryStrategy nfa) (state : SearchState (BufferStrategy bufferSize) nfa) : Prop :=
   state'.states = state.states ∧ refineUpdates state'.updates state.updates
 
-inductive εStack'.refines : εStack' nfa → εStack nfa bufferSize → Prop where
-  | nil : εStack'.refines [] []
+inductive εStack.refines : εStack HistoryStrategy nfa → εStack (BufferStrategy bufferSize) nfa → Prop where
+  | nil : εStack.refines [] []
   | cons {update state' tail' buffer state tail}
-    (h₁ : materializeUpdates bufferSize update = buffer) (h₂ : state' = state) (rest : εStack'.refines tail' tail) :
-    εStack'.refines ((update, state') :: tail') ((buffer, state) :: tail)
+    (h₁ : materializeUpdates bufferSize update = buffer) (h₂ : state' = state) (rest : εStack.refines tail' tail) :
+    εStack.refines ((update, state') :: tail') ((buffer, state) :: tail)
 
 @[simp]
-theorem εStack'.refines_nil : εStack'.refines [] stack ↔ stack = [] :=
+theorem εStack.refines_nil : εStack.refines [] stack ↔ stack = [] :=
   ⟨fun ref => by cases ref; simp, fun h => h ▸ .nil⟩
 
 @[simp]
-theorem εStack'.refines_cons {update state' tail' stack} :
-  @εStack'.refines nfa bufferSize ((update, state') :: tail') stack ↔
-  ∃ buffer state tail, stack = (buffer, state) :: tail ∧ materializeUpdates bufferSize update = buffer ∧ state' = state ∧ @εStack'.refines nfa bufferSize tail' tail := by
+theorem εStack.refines_cons {update state' tail' stack} :
+  @εStack.refines nfa bufferSize ((update, state') :: tail') stack ↔
+  ∃ buffer state tail, stack = (buffer, state) :: tail ∧ materializeUpdates bufferSize update = buffer ∧ state' = state ∧ @εStack.refines nfa bufferSize tail' tail := by
   apply Iff.intro
   . intro ref
     cases ref with
@@ -82,14 +82,14 @@ theorem εStack'.refines_cons {update state' tail' stack} :
   . intro ⟨buffer, state, tail, eq, h₁, h₂, rest⟩
     exact eq ▸ .cons h₁ h₂ rest
 
-theorem εClosure'.refines {result result'}
-  (h : εClosure nfa wf it matched next stack = result)
-  (h' : εClosure' nfa wf it matched' next' stack' = result')
+theorem εClosure.refines {result result'}
+  (h : @εClosure (BufferStrategy bufferSize) nfa wf it matched next stack = result)
+  (h' : @εClosure HistoryStrategy nfa wf it matched' next' stack' = result')
   (refMatched : refineUpdateOpt matched' matched)
   (refState : next'.refines next)
   (refStack : stack'.refines stack) :
   refineUpdateOpt result'.1 result.1 ∧ result'.2.refines result.2 := by
-  induction matched', next', stack' using εClosure'.induct' nfa wf it generalizing matched next stack result result' with
+  induction matched', next', stack' using εClosure.induct' HistoryStrategy nfa wf it generalizing matched next stack result result' with
   | base matched' next' =>
     simp at refStack
     subst stack
@@ -98,70 +98,70 @@ theorem εClosure'.refines {result result'}
   | visited matched' next' update state' stack' mem ih =>
     cases refStack with
     | @cons _ _ tail' buffer state tail h₁ h₂ rest =>
-      rw [εClosure'_visited mem] at h'
-      rw [εClosure_visited (refState.1 ▸ h₂ ▸ mem)] at h
+      rw [εClosure_visited (σ := HistoryStrategy) mem] at h'
+      rw [εClosure_visited (σ := BufferStrategy bufferSize) (refState.1 ▸ h₂ ▸ mem)] at h
       exact ih h h' refMatched refState rest
   | epsilon matched' next' update state' stack' state mem hn next'' =>
     -- TODO: cannot introduce `ih` directly for some reason
     rename_i ih
     cases refStack with
     | @cons _ _ tail' buffer state tail h₁ h₂ rest =>
-      rw [εClosure'_epsilon mem hn] at h'
-      rw [εClosure_epsilon (refState.1 ▸ h₂ ▸ mem) (h₂ ▸ hn)] at h
+      rw [εClosure_epsilon (σ := HistoryStrategy) mem hn] at h'
+      rw [εClosure_epsilon (σ := BufferStrategy bufferSize) (refState.1 ▸ h₂ ▸ mem) (h₂ ▸ hn)] at h
       have : next''.refines ⟨next.states.insert state, next.updates⟩ := by
-        simp [SearchState'.refines, h₂, refState.1, next'']
+        simp [SearchState.refines, h₂, refState.1, next'']
         exact refState.2
       exact ih h h' refMatched this (.cons h₁ rfl rest)
   | anchor_pos matched' next' update state stack' anchor state' mem hn next'' test =>
     rename_i ih
     cases refStack with
     | @cons _ _ tail' buffer state tail h₁ h₂ rest =>
-      rw [εClosure'_anchor_pos mem hn test] at h'
-      rw [εClosure_anchor_pos (refState.1 ▸ h₂ ▸ mem) (h₂ ▸ hn) test] at h
+      rw [εClosure_anchor_pos (σ := HistoryStrategy) mem hn test] at h'
+      rw [εClosure_anchor_pos (σ := BufferStrategy bufferSize) (refState.1 ▸ h₂ ▸ mem) (h₂ ▸ hn) test] at h
       have : next''.refines ⟨next.states.insert state, next.updates⟩ := by
-        simp [SearchState'.refines, h₂, refState.1, next'']
+        simp [SearchState.refines, h₂, refState.1, next'']
         exact refState.2
       exact ih h h' refMatched this (.cons h₁ rfl rest)
   | anchor_neg matched' next' update state stack' anchor state' mem hn next'' test =>
     rename_i ih
     cases refStack with
     | @cons _ _ tail' buffer state tail h₁ h₂ rest =>
-      rw [εClosure'_anchor_neg mem hn test] at h'
-      rw [εClosure_anchor_neg (refState.1 ▸ h₂ ▸ mem) (h₂ ▸ hn) test] at h
+      rw [εClosure_anchor_neg (σ := HistoryStrategy) mem hn test] at h'
+      rw [εClosure_anchor_neg (σ := BufferStrategy bufferSize) (refState.1 ▸ h₂ ▸ mem) (h₂ ▸ hn) test] at h
       have : next''.refines ⟨next.states.insert state, next.updates⟩ := by
-        simp [SearchState'.refines, h₂, refState.1, next'']
+        simp [SearchState.refines, h₂, refState.1, next'']
         exact refState.2
       exact ih h h' refMatched this rest
   | split matched' next' update state stack' state₁ state₂ mem hn next'' =>
     rename_i ih
     cases refStack with
     | @cons _ _ tail' buffer state tail h₁ h₂ rest =>
-      rw [εClosure'_split mem hn] at h'
-      rw [εClosure_split (refState.1 ▸ h₂ ▸ mem) (h₂ ▸ hn)] at h
+      rw [εClosure_split (σ := HistoryStrategy) mem hn] at h'
+      rw [εClosure_split (σ := BufferStrategy bufferSize) (refState.1 ▸ h₂ ▸ mem) (h₂ ▸ hn)] at h
       have : next''.refines ⟨next.states.insert state, next.updates⟩ := by
-        simp [SearchState'.refines, h₂, refState.1, next'']
+        simp [SearchState.refines, h₂, refState.1, next'']
         exact refState.2
       exact ih h h' refMatched this (.cons h₁ rfl (.cons h₁ rfl rest))
   | save matched' next' update state stack' offset state' mem hn next'' =>
     rename_i ih
     cases refStack with
     | @cons _ _ tail' buffer state tail h₁ h₂ rest =>
-      rw [εClosure'_save mem hn] at h'
-      rw [εClosure_save (refState.1 ▸ h₂ ▸ mem) (h₂ ▸ hn)] at h
+      rw [εClosure_save (σ := HistoryStrategy) mem hn] at h'
+      rw [εClosure_save (σ := BufferStrategy bufferSize) (refState.1 ▸ h₂ ▸ mem) (h₂ ▸ hn)] at h
       have : next''.refines ⟨next.states.insert state, next.updates⟩ := by
-        simp [SearchState'.refines, h₂, refState.1, next'']
+        simp [SearchState.refines, h₂, refState.1, next'']
         exact refState.2
-      exact ih h h' refMatched this (.cons (by simp [h₁]) rfl rest)
+      exact ih h h' refMatched this (.cons (by simp [h₁, HistoryStrategy, BufferStrategy]) rfl rest)
   | done matched' next' update state stack' mem hn next'' =>
     rename_i ih
     cases refStack with
     | @cons _ _ tail' buffer state tail h₁ h₂ rest =>
-      rw [εClosure'_done mem hn] at h'
-      rw [εClosure_done (refState.1 ▸ h₂ ▸ mem) (h₂ ▸ hn)] at h
+      rw [εClosure_done (σ := HistoryStrategy) mem hn] at h'
+      rw [εClosure_done (σ := BufferStrategy bufferSize) (refState.1 ▸ h₂ ▸ mem) (h₂ ▸ hn)] at h
       have refMatched' : refineUpdateOpt (matched' <|> some update) (matched <|> some buffer) :=
         refineUpdateOpt.orElse refMatched h₁
       have : next''.refines ⟨next.states.insert state, next.updates.set state buffer⟩ := by
-        simp [SearchState'.refines, h₂, refState.1, next'']
+        simp [SearchState.refines, h₂, refState.1, next'']
         intro i
         if h : state = i then
           simp [h]
@@ -175,10 +175,10 @@ theorem εClosure'.refines {result result'}
     rename_i ih
     cases refStack with
     | @cons _ _ tail' buffer state tail h₁ h₂ rest =>
-      rw [εClosure'_char mem hn] at h'
-      rw [εClosure_char (refState.1 ▸ h₂ ▸ mem) (h₂ ▸ hn)] at h
+      rw [εClosure_char (σ := HistoryStrategy) mem hn] at h'
+      rw [εClosure_char (σ := BufferStrategy bufferSize) (refState.1 ▸ h₂ ▸ mem) (h₂ ▸ hn)] at h
       have : next''.refines ⟨next.states.insert state, next.updates.set state buffer⟩ := by
-        simp [SearchState'.refines, h₂, refState.1, next'']
+        simp [SearchState.refines, h₂, refState.1, next'']
         intro i
         if h : state = i then
           simp [h]
@@ -192,10 +192,10 @@ theorem εClosure'.refines {result result'}
     rename_i ih
     cases refStack with
     | @cons _ _ tail' buffer state tail h₁ h₂ rest =>
-      rw [εClosure'_sparse mem hn] at h'
-      rw [εClosure_sparse (refState.1 ▸ h₂ ▸ mem) (h₂ ▸ hn)] at h
+      rw [εClosure_sparse (σ := HistoryStrategy) mem hn] at h'
+      rw [εClosure_sparse (σ := BufferStrategy bufferSize) (refState.1 ▸ h₂ ▸ mem) (h₂ ▸ hn)] at h
       have : next''.refines ⟨next.states.insert state, next.updates.set state buffer⟩ := by
-        simp [SearchState'.refines, h₂, refState.1, next'']
+        simp [SearchState.refines, h₂, refState.1, next'']
         intro i
         if h : state = i then
           simp [h]
@@ -209,27 +209,27 @@ theorem εClosure'.refines {result result'}
     rename_i ih
     cases refStack with
     | @cons _ _ tail' buffer state tail h₁ h₂ rest =>
-      rw [εClosure'_fail mem hn] at h'
-      rw [εClosure_fail (refState.1 ▸ h₂ ▸ mem) (h₂ ▸ hn)] at h
+      rw [εClosure_fail (σ := HistoryStrategy) mem hn] at h'
+      rw [εClosure_fail (σ := BufferStrategy bufferSize) (refState.1 ▸ h₂ ▸ mem) (h₂ ▸ hn)] at h
       have : next''.refines ⟨next.states.insert state, next.updates⟩ := by
-        simp [SearchState'.refines, h₂, refState.1, next'']
+        simp [SearchState.refines, h₂, refState.1, next'']
         exact refState.2
       exact ih h h' refMatched this rest
 
-theorem stepChar'.refines {currentUpdates currentUpdates' state result result'}
-  (h : stepChar nfa wf it currentUpdates next state = result)
-  (h' : stepChar' nfa wf it currentUpdates' next' state = result')
+theorem stepChar.refines {currentUpdates currentUpdates' state result result'}
+  (h : stepChar (BufferStrategy bufferSize) nfa wf it currentUpdates next state = result)
+  (h' : stepChar HistoryStrategy nfa wf it currentUpdates' next' state = result')
   (refUpdates : refineUpdates currentUpdates' currentUpdates)
   (refState : next'.refines next) :
   refineUpdateOpt result'.1 result.1 ∧ result'.2.refines result.2 := by
-  unfold stepChar' at h'
+  unfold stepChar at h'
   split at h'
   next c state' hn =>
     rw [stepChar_char hn] at h
     split at h'
     next eq =>
       simp [eq] at h h'
-      exact εClosure'.refines h h' (by simp [refineUpdateOpt]) refState (.cons (refUpdates state) rfl .nil)
+      exact εClosure.refines h h' (by simp [refineUpdateOpt]) refState (.cons (refUpdates state) rfl .nil)
     next ne =>
       simp [ne] at h
       simp [←h', ←h, refineUpdateOpt, refState]
@@ -238,7 +238,7 @@ theorem stepChar'.refines {currentUpdates currentUpdates' state result result'}
     split at h'
     next mem =>
       simp [mem] at h h'
-      exact εClosure'.refines h h' (by simp [refineUpdateOpt]) refState (.cons (refUpdates state) rfl .nil)
+      exact εClosure.refines h h' (by simp [refineUpdateOpt]) refState (.cons (refUpdates state) rfl .nil)
     next nmem =>
       simp [nmem] at h
       simp [←h', ←h, refineUpdateOpt, refState]
@@ -246,13 +246,13 @@ theorem stepChar'.refines {currentUpdates currentUpdates' state result result'}
     rw [stepChar_not_char_sparse h₁ h₂] at h
     simp [←h', ←h, refineUpdateOpt, refState]
 
-theorem eachStepChar'.go.refines {current current' i hle hle' result result'}
-  (h : eachStepChar.go nfa wf it current i hle next = result)
-  (h' : eachStepChar'.go nfa wf it current' i hle' next' = result')
+theorem eachStepChar.go.refines {current current' i hle hle' result result'}
+  (h : eachStepChar.go (BufferStrategy bufferSize) nfa wf it current i hle next = result)
+  (h' : eachStepChar.go HistoryStrategy nfa wf it current' i hle' next' = result')
   (refCurrent : current'.refines current)
   (refNext : next'.refines next) :
   refineUpdateOpt result'.1 result.1 ∧ result'.2.refines result.2 := by
-  induction i, hle', next' using eachStepChar'.go.induct' nfa wf it generalizing current next result result' with
+  induction i, hle', next' using eachStepChar.go.induct' HistoryStrategy nfa wf it generalizing current next result result' with
   | base next' =>
     simp at h'
     simp [refCurrent.1] at h
@@ -261,47 +261,47 @@ theorem eachStepChar'.go.refines {current current' i hle hle' result result'}
     have hlt : i < current.states.count := refCurrent.1 ▸ hlt'
     have eq : current.states[i] = current'.states[i] := by
       simp [refCurrent.1]
-    generalize hstep : stepChar nfa wf it current.updates next current.states[i] = stepped
-    have refStepChar := stepChar'.refines hstep (eq ▸ hstep') refCurrent.2 refNext
+    generalize hstep : stepChar (BufferStrategy bufferSize) nfa wf it current.updates next current.states[i] = stepped
+    have refStepChar := stepChar.refines hstep (eq ▸ hstep') refCurrent.2 refNext
     simp at refStepChar
     have isSome : stepped.1.isSome := by
       simp [refineUpdateOpt.isSome_iff refStepChar.1] at isSome'
       exact isSome'
-    rw [eachStepChar'.go_found hlt' hstep' isSome'] at h'
+    rw [eachStepChar.go_found hlt' hstep' isSome'] at h'
     rw [eachStepChar.go_found hlt hstep isSome] at h
     simp [←h', ←h, refStepChar]
   | not_found i hlt' next' matched' next'' hstep' isSome' ih =>
     have hlt : i < current.states.count := refCurrent.1 ▸ hlt'
     have eq : current.states[i] = current'.states[i] := by
       simp [refCurrent.1]
-    generalize hstep : stepChar nfa wf it current.updates next current.states[i] = stepped
-    have refStepChar := stepChar'.refines hstep (eq ▸ hstep') refCurrent.2 refNext
+    generalize hstep : stepChar (BufferStrategy bufferSize) nfa wf it current.updates next current.states[i] = stepped
+    have refStepChar := stepChar.refines hstep (eq ▸ hstep') refCurrent.2 refNext
     simp at refStepChar
     have isSome : ¬stepped.1.isSome := by
       rw [refineUpdateOpt.isSome_iff refStepChar.1] at isSome'
       exact isSome'
-    rw [eachStepChar'.go_not_found hlt' hstep' isSome'] at h'
+    rw [eachStepChar.go_not_found hlt' hstep' isSome'] at h'
     rw [eachStepChar.go_not_found hlt hstep isSome] at h
     exact ih h h' refCurrent refStepChar.2
 
-theorem eachStepChar'.refines {current current' result result'}
-  (h : eachStepChar nfa wf it current next = result)
-  (h' : eachStepChar' nfa wf it current' next' = result')
+theorem eachStepChar.refines {current current' result result'}
+  (h : eachStepChar (BufferStrategy bufferSize) nfa wf it current next = result)
+  (h' : eachStepChar HistoryStrategy nfa wf it current' next' = result')
   (refCurrent : current'.refines current)
   (refNext : next'.refines next) :
   refineUpdateOpt result'.1 result.1 ∧ result'.2.refines result.2 :=
-  eachStepChar'.go.refines h h' refCurrent refNext
+  eachStepChar.go.refines h h' refCurrent refNext
 
-theorem captureNext'.go.refines {current current' result result'}
-  (h : captureNext.go nfa wf bufferSize it matched current next = result)
-  (h' : captureNext'.go nfa wf it matched' current' next' = result')
+theorem captureNext.go.refines {current current' result result'}
+  (h : captureNext.go (BufferStrategy bufferSize) nfa wf it matched current next = result)
+  (h' : captureNext.go HistoryStrategy nfa wf it matched' current' next' = result')
   (refMatched : refineUpdateOpt matched' matched)
   (refCurrent : current'.refines current)
   (refNext : next'.refines next) :
   refineUpdateOpt result' result := by
-  induction it, matched', current', next' using captureNext'.go.induct' nfa wf generalizing matched current next result result' with
+  induction it, matched', current', next' using captureNext.go.induct' HistoryStrategy nfa wf generalizing matched current next result result' with
   | not_found it matched' current' next' atEnd =>
-    rw [captureNext'.go_not_found atEnd] at h'
+    rw [captureNext.go_not_found atEnd] at h'
     rw [captureNext.go_not_found atEnd] at h
     simp [←h', ←h, refMatched]
   | found it matched' current' next' atEnd isEmpty' isSome' =>
@@ -309,48 +309,49 @@ theorem captureNext'.go.refines {current current' result result'}
     have isSome : matched.isSome := by
       rw [refineUpdateOpt.isSome_iff refMatched] at isSome'
       exact isSome'
-    rw [captureNext'.go_found atEnd isEmpty' isSome'] at h'
+    rw [captureNext.go_found atEnd isEmpty' isSome'] at h'
     rw [captureNext.go_found atEnd isEmpty isSome] at h
     simp [←h', ←h, refMatched]
   | ind_not_found it matched' current' next' _ current'' matched'' next'' atEnd isNone' h₁ h₂ ih =>
     have isNone : matched.isNone := by
       rw [refineUpdateOpt.isNone_iff refMatched] at isNone'
       exact isNone'
-    generalize hexpand : εClosure nfa wf it .none current [(Buffer.empty, ⟨nfa.start, wf.start_lt⟩)] = expanded
-    generalize hstep : eachStepChar nfa wf it expanded.2 next = stepped
-    rw [captureNext'.go_ind_not_found atEnd isNone' h₁ h₂] at h'
+    generalize hexpand : εClosure (BufferStrategy bufferSize) nfa wf it .none current [(Buffer.empty, ⟨nfa.start, wf.start_lt⟩)] = expanded
+    generalize hstep : eachStepChar (BufferStrategy bufferSize) nfa wf it expanded.2 next = stepped
+    rw [captureNext.go_ind_not_found atEnd isNone' h₁ h₂] at h'
     rw [captureNext.go_ind_not_found atEnd isNone hexpand hstep] at h
 
-    have refExpanded := εClosure'.refines hexpand h₁ (by simp [refineUpdateOpt]) refCurrent (.cons rfl rfl .nil)
+    have refExpanded := εClosure.refines hexpand h₁ (by simp [refineUpdateOpt]) refCurrent (.cons rfl rfl .nil)
     simp at refExpanded
-    have ⟨refMatched'', refNext''⟩ := eachStepChar'.refines hstep h₂ refExpanded.2 refNext
+    have ⟨refMatched'', refNext''⟩ := eachStepChar.refines hstep h₂ refExpanded.2 refNext
     simp at refMatched'' refNext''
-    exact ih h h' refMatched'' refNext'' (by simp [SearchState'.refines, refExpanded.2.1, refExpanded.2.2])
+    exact ih h h' refMatched'' refNext'' (by simp [SearchState.refines, refExpanded.2.1, refExpanded.2.2])
   | ind_found it matched' current' next' matched'' next'' atEnd isEmpty' isSome' h'' ih =>
     have isEmpty : ¬current.states.isEmpty := refCurrent.1 ▸ isEmpty'
     have isSome : matched.isSome := by
       rw [refineUpdateOpt.isSome_iff refMatched] at isSome'
       exact isSome'
-    generalize hstep : eachStepChar nfa wf it current next = stepped
-    rw [captureNext'.go_ind_found atEnd isEmpty' isSome' h''] at h'
+    generalize hstep : eachStepChar (BufferStrategy bufferSize) nfa wf it current next = stepped
+    simp [BufferStrategy] at stepped
+    rw [captureNext.go_ind_found atEnd isEmpty' isSome' h''] at h'
     rw [captureNext.go_ind_found atEnd isEmpty isSome hstep] at h
 
-    have := eachStepChar'.refines hstep h'' refCurrent refNext
+    have := eachStepChar.refines hstep h'' refCurrent refNext
     simp at this
     have ⟨refMatched'', refNext''⟩ := this
     have : refineUpdateOpt (matched'' <|> matched') (stepped.1 <|> matched) :=
       refineUpdateOpt.orElse refMatched'' refMatched
-    exact ih h h' this refNext'' (by simp [refCurrent.1, SearchState'.refines, refCurrent.2])
+    exact ih h h' this refNext'' (by simp [refCurrent.1, SearchState.refines, refCurrent.2])
 
-theorem captureNext'.refines :
-  refineUpdateOpt (captureNext' nfa wf it) (captureNext nfa wf bufferSize it) := by
-  unfold captureNext' captureNext
+theorem captureNext.refines :
+  refineUpdateOpt (captureNext HistoryStrategy nfa wf it) (captureNext (BufferStrategy bufferSize) nfa wf it) := by
+  unfold captureNext
   simp
-  generalize hexpand' : εClosure' nfa wf it .none ⟨.empty, Vector.mkVector nfa.nodes.size []⟩ [([], ⟨nfa.start, wf.start_lt⟩)] = expanded'
-  generalize hexpand : εClosure nfa wf it .none ⟨.empty, Vector.mkVector nfa.nodes.size Buffer.empty⟩ [(Buffer.empty, ⟨nfa.start, wf.start_lt⟩)] = expanded
+  generalize hexpand' : εClosure HistoryStrategy nfa wf it .none ⟨.empty, Vector.mkVector nfa.nodes.size HistoryStrategy.empty⟩ [(HistoryStrategy.empty, ⟨nfa.start, wf.start_lt⟩)] = expanded'
+  generalize hexpand : εClosure (BufferStrategy bufferSize) nfa wf it .none ⟨.empty, Vector.mkVector nfa.nodes.size (BufferStrategy bufferSize).empty⟩ [((BufferStrategy bufferSize).empty, ⟨nfa.start, wf.start_lt⟩)] = expanded
 
-  have ⟨refMatched, refState⟩ := εClosure'.refines hexpand hexpand'
-    (by simp [refineUpdateOpt]) (by simp [SearchState'.refines, refineUpdates]) (.cons rfl rfl .nil)
-  exact captureNext'.go.refines rfl rfl refMatched refState (by simp [SearchState'.refines, refineUpdates])
+  have ⟨refMatched, refState⟩ := εClosure.refines hexpand hexpand'
+    (by simp [refineUpdateOpt]) (by simp [SearchState.refines, refineUpdates]) (.cons rfl rfl .nil)
+  exact captureNext.go.refines rfl rfl refMatched refState (by simp [SearchState.refines, refineUpdates])
 
 end Regex.VM
