regex/Regex/VM/Strategy.lean
@@ -8,7 +8,7 @@ open String (Pos)
 
 namespace Regex.VM
 
-class Strategy where
+structure Strategy where
   Update : Type
   empty : Update
   write : Update → Nat → Pos → Update
@@ -27,5 +27,22 @@ def BufferStrategy (size : Nat) : Strategy where
   Update := Buffer size
   empty := Buffer.empty
   write buffer offset pos := Vector.setIfInBounds buffer offset pos
+
+instance {size} : Repr (BufferStrategy size).Update := inferInstanceAs (Repr (Vector (Option Pos) size))
+
+instance {size} : Inhabited (BufferStrategy size).Update := inferInstanceAs (Inhabited (Vector (Option Pos) size))
+
+instance {size} : DecidableEq (BufferStrategy size).Update := inferInstanceAs (DecidableEq (Vector (Option Pos) size))
+
+instance {size} : GetElem (BufferStrategy size).Update Nat (Option Pos) (fun _ i => i < size) :=
+  inferInstanceAs (GetElem (Vector (Option Pos) size) Nat (Option Pos) _)
+
+/--
+This strategy is used only for proofs and inefficient.
+-/
+def HistoryStrategy : Strategy where
+  Update := List (Nat × Pos)
+  empty := []
+  write update offset pos := update ++ [(offset, pos)]
 
 end Regex.VM
