correctness/RegexCorrectness/Regex/Captures.lean
@@ -26,13 +26,14 @@ namespace Regex.Captures
 def Valid (self : Captures) : Prop :=
   self.regex.IsSearchRegex ∧ self.currentPos.Valid self.haystack
 
+-- TODO: what to do when self.currentPos = self.haystack.endPos?
 theorem captures_of_next?_some {self self' : Captures} {captured} (h : self.next? = .some (captured, self'))
   (v : self.Valid) :
   self'.Valid ∧ captured.Spec v.1 self.haystack := by
   unfold next? at h
   split at h
   next lt =>
-    generalize h' : VM.captureNext self.regex.nfa self.regex.wf (self.regex.maxTag + 1) ⟨self.haystack, self.currentPos⟩ = matched at h
+    generalize h' : VM.captureNextBuf self.regex.nfa self.regex.wf (self.regex.maxTag + 1) ⟨self.haystack, self.currentPos⟩ = matched at h
     match matched with
     | none => simp at h
     | some matched =>
@@ -91,6 +92,7 @@ theorem captures_of_next?_some {self self' : Captures} {captured} (h : self.next
         simp [hcaptured 0]
         have h₁ := (eqv 0).1 (by omega)
         have h₂ := (eqv 0).2 (by omega)
+        simp [VM.BufferStrategy] at eq₁ eq₂
         simp [eq₁] at h₁
         simp [eq₂] at h₂
         have ⟨_, eq₁⟩ := h₁
@@ -109,7 +111,7 @@ theorem captures_of_next?_some {self self' : Captures} {captured} (h : self.next
       next nlt =>
         simp at h
         simp [←h, Valid]
-        exact ⟨⟨v.1, String.valid_next v.2 lt⟩, l, m, r, groups, by simp [eqstring], c, captured₀, hcaptured⟩
+        exact ⟨⟨v.1, String.valid_next v.2 sorry⟩, l, m, r, groups, by simp [eqstring], c, captured₀, hcaptured⟩
   next => simp at h
 
 theorem regex_eq_of_next?_some {self self' : Captures} {captured} (h : self.next? = .some (captured, self')) :
@@ -118,7 +120,7 @@ theorem regex_eq_of_next?_some {self self' : Captures} {captured} (h : self.next
   split at h
   next =>
     simp at h
-    set captured' := VM.captureNext self.regex.nfa self.regex.wf (self.regex.maxTag + 1) ⟨self.haystack, self.currentPos⟩
+    set captured' := VM.captureNextBuf self.regex.nfa self.regex.wf (self.regex.maxTag + 1) ⟨self.haystack, self.currentPos⟩
     match h' : captured' with
     | none => simp at h
     | some buffer =>
@@ -142,7 +144,7 @@ theorem haystack_eq_of_next?_some {self self' : Captures} {captured} (h : self.n
   split at h
   next =>
     simp at h
-    set captured' := VM.captureNext self.regex.nfa self.regex.wf (self.regex.maxTag + 1) ⟨self.haystack, self.currentPos⟩
+    set captured' := VM.captureNextBuf self.regex.nfa self.regex.wf (self.regex.maxTag + 1) ⟨self.haystack, self.currentPos⟩
     match h' : captured' with
     | none => simp at h
     | some buffer =>
