correctness/RegexCorrectness/VM/EpsilonClosure/Basic.lean
@@ -1,6 +1,7 @@
 import Regex.Data.SparseSet
 import Regex.NFA.Basic
 import Regex.VM
+import Regex.VM.Strategy
 import RegexCorrectness.VM.Path
 
 set_option autoImplicit false
@@ -11,258 +12,212 @@ open String (Pos Iterator)
 
 namespace Regex.VM
 
-abbrev εStack' (nfa : NFA) := List (List (Nat × Pos) × Fin nfa.nodes.size)
-
-/--
-A version of εClosure traversal that tracks the updates to the capture groups.
-
-As the NFA semantics use `List (Nat × Pos)` to represent the capture group updates, this
-εClosure implementation also use it for verification. The actual VM implementation materializes the
-updates as a `Buffer` for efficiency, and the correspondence will be proved in `Correspondence.lean`.
--/
-def εClosure' (nfa : NFA) (wf : nfa.WellFormed) (it : Iterator)
-  (matched : Option (List (Nat × Pos))) (next : SearchState' nfa) (stack : εStack' nfa) :
-  Option (List (Nat × Pos)) × SearchState' nfa :=
-  match stack with
-  | [] => (matched, next)
-  | (update, state) :: stack' =>
-    if state ∈ next.states then
-      εClosure' nfa wf it matched next stack'
-    else
-      let states' := next.states.insert state
-      match hn : nfa[state] with
-      | .epsilon state' =>
-        have isLt : state' < nfa.nodes.size := wf.inBounds' state hn
-        εClosure' nfa wf it matched ⟨states', next.updates⟩ ((update, ⟨state', isLt⟩) :: stack')
-      | .anchor anchor state' =>
-        have isLt : state' < nfa.nodes.size := wf.inBounds' state hn
-        if anchor.test it then
-          εClosure' nfa wf it matched ⟨states', next.updates⟩ ((update, ⟨state', isLt⟩) :: stack')
-        else
-          εClosure' nfa wf it matched ⟨states', next.updates⟩ stack'
-      | .split state₁ state₂ =>
-        have isLt : state₁ < nfa.nodes.size ∧ state₂ < nfa.nodes.size := wf.inBounds' state hn
-        εClosure' nfa wf it matched ⟨states', next.updates⟩ ((update, ⟨state₁, isLt.1⟩) :: (update, ⟨state₂, isLt.2⟩):: stack')
-      | .save offset state' =>
-        have isLt : state' < nfa.nodes.size := wf.inBounds' state hn
-        let update' := update ++ [(offset, it.pos)]
-        εClosure' nfa wf it matched ⟨states', next.updates⟩ ((update', ⟨state', isLt⟩) :: stack')
-      | .done =>
-        let matched' := matched <|> update
-        let updates' := next.updates.set state update
-        εClosure' nfa wf it matched' ⟨states', updates'⟩ stack'
-      | .char c state' =>
-        let updates' := next.updates.set state update
-        εClosure' nfa wf it matched ⟨states', updates'⟩ stack'
-      | .sparse cs state' =>
-        let updates' := next.updates.set state update
-        εClosure' nfa wf it matched ⟨states', updates'⟩ stack'
-      | .fail => εClosure' nfa wf it matched ⟨states', next.updates⟩ stack'
-termination_by (next.states.measure, stack)
-
 -- Cleaner version of the fuction induction principle
 -- It's crucial to annotate the types of the arguments of the branches. Otherwise, Lean consumse
 -- too much memory. See https://github.com/leanprover/lean4/issues/6753.
-theorem εClosure'.induct' (nfa : NFA) (wf : nfa.WellFormed) (it : Iterator)
-  (motive : Option (List (Nat × Pos)) → SearchState' nfa → εStack' nfa → Prop)
-  (base : ∀ (matched : Option (List (Nat × Pos))) (next : SearchState' nfa), motive matched next [])
+theorem εClosure.induct' (σ : Strategy) (nfa : NFA) (wf : nfa.WellFormed) (it : Iterator)
+  (motive : Option σ.Update → SearchState σ nfa → εStack σ nfa → Prop)
+  (base : ∀ (matched : Option σ.Update) (next : SearchState σ nfa), motive matched next [])
   (visited :
-    ∀ (matched : Option (List (Nat × Pos))) (next : SearchState' nfa) (update : List (Nat × Pos))
-      (state : Fin nfa.nodes.size) (stack' : εStack' nfa),
+    ∀ (matched : Option σ.Update) (next : SearchState σ nfa) (update : σ.Update)
+      (state : Fin nfa.nodes.size) (stack' : εStack σ nfa),
     state ∈ next.states →
     motive matched next stack' →
     motive matched next ((update, state) :: stack'))
   (epsilon :
-    ∀ (matched : Option (List (Nat × Pos))) (next : SearchState' nfa) (update : List (Nat × Pos))
-      (state : Fin nfa.nodes.size) (stack' : εStack' nfa) (state' : Fin nfa.nodes.size),
+    ∀ (matched : Option σ.Update) (next : SearchState σ nfa) (update : σ.Update)
+      (state : Fin nfa.nodes.size) (stack' : εStack σ nfa) (state' : Fin nfa.nodes.size),
     state ∉ next.states → nfa[state] = .epsilon state' →
-    let next' : SearchState' nfa := ⟨next.states.insert state, next.updates⟩;
+    let next' : SearchState σ nfa := ⟨next.states.insert state, next.updates⟩;
     motive matched next' ((update, state') :: stack') →
     motive matched next ((update, state) :: stack'))
   (anchor_pos :
-    ∀ (matched : Option (List (Nat × Pos))) (next : SearchState' nfa) (update : List (Nat × Pos))
-      (state : Fin nfa.nodes.size) (stack' : εStack' nfa) (anchor : Data.Anchor) (state' : Fin nfa.nodes.size),
+    ∀ (matched : Option σ.Update) (next : SearchState σ nfa) (update : σ.Update)
+      (state : Fin nfa.nodes.size) (stack' : εStack σ nfa) (anchor : Data.Anchor) (state' : Fin nfa.nodes.size),
     state ∉ next.states → nfa[state] = .anchor anchor state' →
-    let next' : SearchState' nfa := ⟨next.states.insert state, next.updates⟩;
+    let next' : SearchState σ nfa := ⟨next.states.insert state, next.updates⟩;
     anchor.test it →
     motive matched next' ((update, state') :: stack') →
     motive matched next ((update, state) :: stack'))
   (anchor_neg :
-    ∀ (matched : Option (List (Nat × Pos))) (next : SearchState' nfa) (update : List (Nat × Pos))
-      (state : Fin nfa.nodes.size) (stack' : εStack' nfa) (anchor : Data.Anchor) (state' : Fin nfa.nodes.size),
+    ∀ (matched : Option σ.Update) (next : SearchState σ nfa) (update : σ.Update)
+      (state : Fin nfa.nodes.size) (stack' : εStack σ nfa) (anchor : Data.Anchor) (state' : Fin nfa.nodes.size),
     state ∉ next.states → nfa[state] = .anchor anchor state' →
-    let next' : SearchState' nfa := ⟨next.states.insert state, next.updates⟩;
+    let next' : SearchState σ nfa := ⟨next.states.insert state, next.updates⟩;
     ¬anchor.test it →
     motive matched next' stack' →
     motive matched next ((update, state) :: stack'))
   (split :
-    ∀ (matched : Option (List (Nat × Pos))) (next : SearchState' nfa) (update : List (Nat × Pos))
-      (state : Fin nfa.nodes.size) (stack' : εStack' nfa) (state₁ : Fin nfa.nodes.size) (state₂ : Fin nfa.nodes.size),
+    ∀ (matched : Option σ.Update) (next : SearchState σ nfa) (update : σ.Update)
+      (state : Fin nfa.nodes.size) (stack' : εStack σ nfa) (state₁ : Fin nfa.nodes.size) (state₂ : Fin nfa.nodes.size),
     state ∉ next.states → nfa[state] = .split state₁ state₂ →
-    let next' : SearchState' nfa := ⟨next.states.insert state, next.updates⟩;
+    let next' : SearchState σ nfa := ⟨next.states.insert state, next.updates⟩;
     motive matched next' ((update, state₁) :: (update, state₂) :: stack') →
     motive matched next ((update, state) :: stack'))
   (save :
-    ∀ (matched : Option (List (Nat × Pos))) (next : SearchState' nfa) (update : List (Nat × Pos))
-      (state : Fin nfa.nodes.size) (stack' : εStack' nfa) (offset : Nat) (state' : Fin nfa.nodes.size),
+    ∀ (matched : Option σ.Update) (next : SearchState σ nfa) (update : σ.Update)
+      (state : Fin nfa.nodes.size) (stack' : εStack σ nfa) (offset : Nat) (state' : Fin nfa.nodes.size),
     state ∉ next.states → nfa[state] = .save offset state' →
-    let next' : SearchState' nfa := ⟨next.states.insert state, next.updates⟩;
-    motive matched next' ((update ++ [(offset, it.pos)], state') :: stack') →
+    let next' : SearchState σ nfa := ⟨next.states.insert state, next.updates⟩;
+    motive matched next' ((σ.write update offset it.pos, state') :: stack') →
     motive matched next ((update, state) :: stack'))
   (done :
-    ∀ (matched : Option (List (Nat × Pos))) (next : SearchState' nfa) (update : List (Nat × Pos))
-      (state : Fin nfa.nodes.size) (stack' : εStack' nfa),
+    ∀ (matched : Option σ.Update) (next : SearchState σ nfa) (update : σ.Update)
+      (state : Fin nfa.nodes.size) (stack' : εStack σ nfa),
     state ∉ next.states → nfa[state] = .done →
-    let next' : SearchState' nfa := ⟨next.states.insert state, next.updates.set state update⟩;
+    let next' : SearchState σ nfa := ⟨next.states.insert state, next.updates.set state update⟩;
     motive (matched <|> .some update) next' stack' →
     motive matched next ((update, state) :: stack'))
   (char :
-    ∀ (matched : Option (List (Nat × Pos))) (next : SearchState' nfa) (update : List (Nat × Pos))
-      (state : Fin nfa.nodes.size) (stack' : εStack' nfa) (c : Char) (state' : Fin nfa.nodes.size),
+    ∀ (matched : Option σ.Update) (next : SearchState σ nfa) (update : σ.Update)
+      (state : Fin nfa.nodes.size) (stack' : εStack σ nfa) (c : Char) (state' : Fin nfa.nodes.size),
     state ∉ next.states → nfa[state] = .char c state' →
-    let next' : SearchState' nfa := ⟨next.states.insert state, next.updates.set state update⟩;
+    let next' : SearchState σ nfa := ⟨next.states.insert state, next.updates.set state update⟩;
     motive matched next' stack' →
     motive matched next ((update, state) :: stack'))
   (sparse :
-    ∀ (matched : Option (List (Nat × Pos))) (next : SearchState' nfa) (update : List (Nat × Pos))
-      (state : Fin nfa.nodes.size) (stack' : εStack' nfa) (cs : Data.Classes) (state' : Fin nfa.nodes.size),
+    ∀ (matched : Option σ.Update) (next : SearchState σ nfa) (update : σ.Update)
+      (state : Fin nfa.nodes.size) (stack' : εStack σ nfa) (cs : Data.Classes) (state' : Fin nfa.nodes.size),
     state ∉ next.states → nfa[state] = .sparse cs state' →
-    let next' : SearchState' nfa := ⟨next.states.insert state, next.updates.set state update⟩;
+    let next' : SearchState σ nfa := ⟨next.states.insert state, next.updates.set state update⟩;
     motive matched next' stack' →
     motive matched next ((update, state) :: stack'))
   (fail :
-    ∀ (matched : Option (List (Nat × Pos))) (next : SearchState' nfa) (update : List (Nat × Pos))
-      (state : Fin nfa.nodes.size) (stack' : εStack' nfa),
+    ∀ (matched : Option σ.Update) (next : SearchState σ nfa) (update : σ.Update)
+      (state : Fin nfa.nodes.size) (stack' : εStack σ nfa),
     state ∉ next.states → nfa[state] = .fail →
-    let next' : SearchState' nfa := ⟨next.states.insert state, next.updates⟩;
+    let next' : SearchState σ nfa := ⟨next.states.insert state, next.updates⟩;
     motive matched next' stack' →
     motive matched next ((update, state) :: stack')) :
   ∀ matched next stack, motive matched next stack := fun matched next stack =>
-    εClosure'.induct nfa wf it motive base visited
-      (fun matched next update state stack' mem state' hn isLt ih =>
-        epsilon matched next update state stack' ⟨state', isLt⟩ mem hn ih)
-      (fun matched next update state stack' mem a state' hn isLt h ih =>
-        anchor_pos matched next update state stack' a ⟨state', isLt⟩ mem hn h ih)
-      (fun matched next update state stack' mem a state' hn isLt h ih =>
-        anchor_neg matched next update state stack' a ⟨state', isLt⟩ mem hn h ih)
-      (fun matched next update state stack' mem state₁ state₂ hn isLt ih =>
-        split matched next update state stack' ⟨state₁, isLt.1⟩ ⟨state₂, isLt.2⟩ mem hn ih)
-      (fun matched next update state stack' mem offset state' hn isLt ih =>
-        save matched next update state stack' offset ⟨state', isLt⟩ mem hn ih)
-      (fun matched next update state stack' mem hn ih =>
-        done matched next update state stack' mem hn ih)
-      (fun matched next update state stack' mem c state' hn ih =>
-        char matched next update state stack' c ⟨state', wf.inBounds' state hn⟩ mem hn ih)
-      (fun matched next update state stack' mem cs state' hn ih =>
-        sparse matched next update state stack' cs ⟨state', wf.inBounds' state hn⟩ mem hn ih)
-      (fun matched next update state stack' mem hn ih =>
-        fail matched next update state stack' mem hn ih)
+    εClosure.induct σ nfa wf it motive base visited
+      (fun matched update state stack' states updates state' hn isLt mem ih =>
+        epsilon matched ⟨states, updates⟩ update state stack' ⟨state', isLt⟩ mem hn ih)
+      (fun matched update state stack' states updates anchor state' hn isLt test mem ih =>
+        anchor_pos matched ⟨states, updates⟩ update state stack' anchor ⟨state', isLt⟩ mem hn test ih)
+      (fun matched update state stack' states updates anchor state' hn isLt test mem ih =>
+        anchor_neg matched ⟨states, updates⟩ update state stack' anchor ⟨state', isLt⟩ mem hn test ih)
+      (fun matched update state stack' states updates state₁ state₂ hn isLt mem ih =>
+        split matched ⟨states, updates⟩ update state stack' ⟨state₁, isLt.1⟩ ⟨state₂, isLt.2⟩ mem hn ih)
+      (fun matched update state stack' states updates offset state' hn isLt mem ih =>
+        save matched ⟨states, updates⟩ update state stack' offset ⟨state', isLt⟩ mem hn ih)
+      (fun matched update state stack' states updates hn mem ih =>
+        done matched ⟨states, updates⟩ update state stack' mem hn ih)
+      (fun matched update state stack' states updates c state' hn mem ih =>
+        char matched ⟨states, updates⟩ update state stack' c ⟨state', wf.inBounds' state hn⟩ mem hn ih)
+      (fun matched update state stack' states updates cs state' hn mem ih =>
+        sparse matched ⟨states, updates⟩ update state stack' cs ⟨state', wf.inBounds' state hn⟩ mem hn ih)
+      (fun matched update state stack' states updates hn mem ih =>
+        fail matched ⟨states, updates⟩ update state stack' mem hn ih)
       matched next stack
 
 /-
-Simplification lemmas for `εClosure'`.
+Simplification lemmas for `εClosure`.
 -/
 section
 
-variable {nfa wf it matched next}
+variable {σ nfa wf it matched next}
 
 @[simp]
-theorem εClosure'_base : εClosure' nfa wf it matched next [] = (matched, next) := by
-  simp [εClosure']
+theorem εClosure_base : εClosure σ nfa wf it matched next [] = (matched, next) := by
+  simp [εClosure]
 
 @[simp]
-theorem εClosure'_visited {update state stack'} (hmem : state ∈ next.states) :
-  εClosure' nfa wf it matched next ((update, state) :: stack') =
-  εClosure' nfa wf it matched next stack' := by
-  simp [εClosure', hmem]
-
-@[simp]
-theorem εClosure'_epsilon {update state stack' state'} (hmem : state ∉ next.states) (hn : nfa[state] = .epsilon state') :
-  εClosure' nfa wf it matched next ((update, state) :: stack') =
-  εClosure' nfa wf it matched ⟨next.states.insert state, next.updates⟩ ((update, state') :: stack') := by
+theorem εClosure_visited {update state stack'} (hmem : state ∈ next.states) :
+  εClosure σ nfa wf it matched next ((update, state) :: stack') =
+  εClosure σ nfa wf it matched next stack' := by
   conv =>
     lhs
-    unfold εClosure'
+    unfold εClosure
+    simp [hmem]
+
+@[simp]
+theorem εClosure_epsilon {update state stack' state'} (hmem : state ∉ next.states) (hn : nfa[state] = .epsilon state') :
+  εClosure σ nfa wf it matched next ((update, state) :: stack') =
+  εClosure σ nfa wf it matched ⟨next.states.insert state, next.updates⟩ ((update, state') :: stack') := by
+  conv =>
+    lhs
+    unfold εClosure
     simp [hmem]
   split <;> simp_all
 
 @[simp]
-theorem εClosure'_anchor_pos {update state stack' anchor state'} (hmem : state ∉ next.states) (hn : nfa[state] = .anchor anchor state') (h : anchor.test it) :
-  εClosure' nfa wf it matched next ((update, state) :: stack') =
-  εClosure' nfa wf it matched ⟨next.states.insert state, next.updates⟩ ((update, state') :: stack') := by
+theorem εClosure_anchor_pos {update state stack' anchor state'} (hmem : state ∉ next.states) (hn : nfa[state] = .anchor anchor state') (h : anchor.test it) :
+  εClosure σ nfa wf it matched next ((update, state) :: stack') =
+  εClosure σ nfa wf it matched ⟨next.states.insert state, next.updates⟩ ((update, state') :: stack') := by
   conv =>
     lhs
-    unfold εClosure'
+    unfold εClosure
     simp [hmem]
   split <;> simp_all
 
 @[simp]
-theorem εClosure'_anchor_neg {update state stack' anchor state'} (hmem : state ∉ next.states) (hn : nfa[state] = .anchor anchor state') (h : ¬anchor.test it) :
-  εClosure' nfa wf it matched next ((update, state) :: stack') =
-  εClosure' nfa wf it matched ⟨next.states.insert state, next.updates⟩ stack' := by
+theorem εClosure_anchor_neg {update state stack' anchor state'} (hmem : state ∉ next.states) (hn : nfa[state] = .anchor anchor state') (h : ¬anchor.test it) :
+  εClosure σ nfa wf it matched next ((update, state) :: stack') =
+  εClosure σ nfa wf it matched ⟨next.states.insert state, next.updates⟩ stack' := by
   conv =>
     lhs
-    unfold εClosure'
+    unfold εClosure
     simp [hmem]
   split <;> simp_all
 
 @[simp]
-theorem εClosure'_split {update state stack' state₁ state₂} (hmem : state ∉ next.states) (hn : nfa[state] = .split state₁ state₂) :
-  εClosure' nfa wf it matched next ((update, state) :: stack') =
-  εClosure' nfa wf it matched ⟨next.states.insert state, next.updates⟩ ((update, state₁) :: (update, state₂) :: stack') := by
+theorem εClosure_split {update state stack' state₁ state₂} (hmem : state ∉ next.states) (hn : nfa[state] = .split state₁ state₂) :
+  εClosure σ nfa wf it matched next ((update, state) :: stack') =
+  εClosure σ nfa wf it matched ⟨next.states.insert state, next.updates⟩ ((update, state₁) :: (update, state₂) :: stack') := by
   conv =>
     lhs
-    unfold εClosure'
+    unfold εClosure
     simp [hmem]
   split <;> simp_all
 
 @[simp]
-theorem εClosure'_save {update state stack' offset state'} (hmem : state ∉ next.states) (hn : nfa[state] = .save offset state') :
-  εClosure' nfa wf it matched next ((update, state) :: stack') =
-  εClosure' nfa wf it matched ⟨next.states.insert state, next.updates⟩ ((update ++ [(offset, it.pos)], state') :: stack') := by
+theorem εClosure_save {update state stack' offset state'} (hmem : state ∉ next.states) (hn : nfa[state] = .save offset state') :
+  εClosure σ nfa wf it matched next ((update, state) :: stack') =
+  εClosure σ nfa wf it matched ⟨next.states.insert state, next.updates⟩ ((σ.write update offset it.pos, state') :: stack') := by
   conv =>
     lhs
-    unfold εClosure'
+    unfold εClosure
     simp [hmem]
   split <;> simp_all
 
 @[simp]
-theorem εClosure'_done {update state stack'} (hmem : state ∉ next.states) (hn : nfa[state] = .done) :
-  εClosure' nfa wf it matched next ((update, state) :: stack') =
-  εClosure' nfa wf it (matched <|> .some update) ⟨next.states.insert state, next.updates.set state update⟩ stack' := by
+theorem εClosure_done {update state stack'} (hmem : state ∉ next.states) (hn : nfa[state] = .done) :
+  εClosure σ nfa wf it matched next ((update, state) :: stack') =
+  εClosure σ nfa wf it (matched <|> .some update) ⟨next.states.insert state, next.updates.set state update⟩ stack' := by
   conv =>
     lhs
-    unfold εClosure'
+    unfold εClosure
     simp [hmem]
   split <;> simp_all
 
 @[simp]
-theorem εClosure'_char {update state stack' c state'} (hmem : state ∉ next.states) (hn : nfa[state] = .char c state') :
-  εClosure' nfa wf it matched next ((update, state) :: stack') =
-  εClosure' nfa wf it matched ⟨next.states.insert state, next.updates.set state update⟩ stack' := by
+theorem εClosure_char {update state stack' c state'} (hmem : state ∉ next.states) (hn : nfa[state] = .char c state') :
+  εClosure σ nfa wf it matched next ((update, state) :: stack') =
+  εClosure σ nfa wf it matched ⟨next.states.insert state, next.updates.set state update⟩ stack' := by
   conv =>
     lhs
-    unfold εClosure'
+    unfold εClosure
     simp [hmem]
   split <;> simp_all
 
 @[simp]
-theorem εClosure'_sparse {update state stack' cs state'} (hmem : state ∉ next.states) (hn : nfa[state] = .sparse cs state') :
-  εClosure' nfa wf it matched next ((update, state) :: stack') =
-  εClosure' nfa wf it matched ⟨next.states.insert state, next.updates.set state update⟩ stack' := by
+theorem εClosure_sparse {update state stack' cs state'} (hmem : state ∉ next.states) (hn : nfa[state] = .sparse cs state') :
+  εClosure σ nfa wf it matched next ((update, state) :: stack') =
+  εClosure σ nfa wf it matched ⟨next.states.insert state, next.updates.set state update⟩ stack' := by
   conv =>
     lhs
-    unfold εClosure'
+    unfold εClosure
     simp [hmem]
   split <;> simp_all
 
 @[simp]
-theorem εClosure'_fail {update state stack'} (hmem : state ∉ next.states) (hn : nfa[state] = .fail) :
-  εClosure' nfa wf it matched next ((update, state) :: stack') =
-  εClosure' nfa wf it matched ⟨next.states.insert state, next.updates⟩ stack' := by
+theorem εClosure_fail {update state stack'} (hmem : state ∉ next.states) (hn : nfa[state] = .fail) :
+  εClosure σ nfa wf it matched next ((update, state) :: stack') =
+  εClosure σ nfa wf it matched ⟨next.states.insert state, next.updates⟩ stack' := by
   conv =>
     lhs
-    unfold εClosure'
+    unfold εClosure
     simp [hmem]
   split <;> simp_all
 
