correctness/RegexCorrectness/VM/Search/Basic.lean
@@ -10,29 +10,8 @@ open String (Pos Iterator)
 
 namespace Regex.VM
 
-def captureNext' (nfa : NFA) (wf : nfa.WellFormed) (it : Iterator) : Option (List (Nat × Pos)) :=
-  let updates := Vector.mkVector nfa.nodes.size []
-  let (matched, current) := εClosure' nfa wf it .none ⟨.empty, updates⟩ [([], ⟨nfa.start, wf.start_lt⟩)]
-  go it matched current ⟨.empty, updates⟩
-where
-  go (it : Iterator) (matched : Option (List (Nat × Pos))) (current next : SearchState' nfa) :
-    Option (List (Nat × String.Pos)) :=
-    if it.atEnd then
-      matched
-    else
-      if current.states.isEmpty && matched.isSome then
-        matched
-      else
-        if matched.isNone then
-          let expanded := εClosure' nfa wf it .none current [([], ⟨nfa.start, wf.start_lt⟩)]
-          let stepped := eachStepChar' nfa wf it expanded.2 next
-          go it.next stepped.1 stepped.2 ⟨expanded.2.states.clear, expanded.2.updates⟩
-        else
-          let stepped := eachStepChar' nfa wf it current next
-          go it.next (stepped.1 <|> matched) stepped.2 ⟨current.states.clear, current.updates⟩
-
-theorem captureNext'.go.induct' (nfa : NFA) (wf : nfa.WellFormed)
-  (motive : Iterator → Option (List (Nat × Pos)) → SearchState' nfa → SearchState' nfa → Prop)
+theorem captureNext.go.induct' (σ : Strategy) (nfa : NFA) (wf : nfa.WellFormed)
+  (motive : Iterator → Option σ.Update → SearchState σ nfa → SearchState σ nfa → Prop)
   (not_found : ∀ it matched current next,
     it.atEnd →
     motive it matched current next)
@@ -41,28 +20,28 @@ theorem captureNext'.go.induct' (nfa : NFA) (wf : nfa.WellFormed)
     motive it matched current next)
   (ind_not_found : ∀ it matched current next _matched current' matched' next',
     ¬it.atEnd → matched.isNone →
-    εClosure' nfa wf it .none current [([], ⟨nfa.start, wf.start_lt⟩)] = (_matched, current') →
-    eachStepChar' nfa wf it current' next = (matched', next') →
+    εClosure σ nfa wf it .none current [(σ.empty, ⟨nfa.start, wf.start_lt⟩)] = (_matched, current') →
+    eachStepChar σ nfa wf it current' next = (matched', next') →
     motive it.next matched' next' ⟨current'.states.clear, current'.updates⟩ →
     motive it matched current next)
   (ind_found : ∀ it matched current next matched' next',
     ¬it.atEnd → ¬current.states.isEmpty → matched.isSome →
-    eachStepChar' nfa wf it current next = (matched', next') →
+    eachStepChar σ nfa wf it current next = (matched', next') →
     motive it.next (matched' <|> matched) next' ⟨current.states.clear, current.updates⟩ →
     motive it matched current next)
-  (it : Iterator) (matched : Option (List (Nat × Pos))) (current next : SearchState' nfa) :
+  (it : Iterator) (matched : Option σ.Update) (current next : SearchState σ nfa) :
   motive it matched current next :=
-  captureNext'.go.induct nfa wf motive
+  captureNext.go.induct σ nfa wf motive
     (fun it matched current next atEnd => not_found it matched current next atEnd)
     (fun it matched current next atEnd h =>
       found it matched current next atEnd (by simp at h; exact h.1) (by simp at h; exact h.2))
     (fun it matched current next atEnd h isNone ih =>
-      let expanded := εClosure' nfa wf it .none current [([], ⟨nfa.start, wf.start_lt⟩)]
-      let stepped := eachStepChar' nfa wf it expanded.2 next
+      let expanded := εClosure σ nfa wf it .none current [(σ.empty, ⟨nfa.start, wf.start_lt⟩)]
+      let stepped := eachStepChar σ nfa wf it expanded.2 next
       ind_not_found it matched current next expanded.1 expanded.2 stepped.1 stepped.2
         atEnd isNone rfl rfl ih)
     (fun it matched current next atEnd h isSome ih =>
-      let stepped := eachStepChar' nfa wf it current next
+      let stepped := eachStepChar σ nfa wf it current next
       ind_found it matched current next stepped.1 stepped.2
         atEnd (by simp at isSome; simp [isSome] at h; simp [h]) (by cases matched <;> simp at isSome; simp) rfl ih)
     it matched current next
@@ -70,39 +49,39 @@ theorem captureNext'.go.induct' (nfa : NFA) (wf : nfa.WellFormed)
 section
 
 @[simp]
-theorem captureNext'.go_not_found {nfa wf it matched current next} (atEnd : it.atEnd) :
-  captureNext'.go nfa wf it matched current next = matched := by
-  simp [captureNext'.go, atEnd]
+theorem captureNext.go_not_found {σ nfa wf it matched current next} (atEnd : it.atEnd) :
+  captureNext.go σ nfa wf it matched current next = matched := by
+  simp [captureNext.go, atEnd]
 
 @[simp]
-theorem captureNext'.go_found {nfa wf it matched current next}
+theorem captureNext.go_found {σ nfa wf it matched current next}
   (atEnd : ¬it.atEnd) (isEmpty : current.states.isEmpty) (isSome : matched.isSome) :
-  captureNext'.go nfa wf it matched current next = matched := by
-  simp [captureNext'.go, atEnd, isEmpty, isSome]
+  captureNext.go σ nfa wf it matched current next = matched := by
+  simp [captureNext.go, atEnd, isEmpty, isSome]
 
 @[simp]
-theorem captureNext'.go_ind_not_found {nfa wf it matched current next _matched current' matched' next'}
+theorem captureNext.go_ind_not_found {σ nfa wf it matched current next _matched current' matched' next'}
   (atEnd : ¬it.atEnd) (isNone : matched.isNone)
-  (h₁ : εClosure' nfa wf it .none current [([], ⟨nfa.start, wf.start_lt⟩)] = (_matched, current'))
-  (h₂ : eachStepChar' nfa wf it current' next = (matched', next')) :
-  captureNext'.go nfa wf it matched current next = captureNext'.go nfa wf it.next matched' next' ⟨current'.states.clear, current'.updates⟩ := by
+  (h₁ : εClosure σ nfa wf it .none current [(σ.empty, ⟨nfa.start, wf.start_lt⟩)] = (_matched, current'))
+  (h₂ : eachStepChar σ nfa wf it current' next = (matched', next')) :
+  captureNext.go σ nfa wf it matched current next = captureNext.go σ nfa wf it.next matched' next' ⟨current'.states.clear, current'.updates⟩ := by
   have isSome : ¬matched.isSome := by
     cases matched <;> simp_all
   conv =>
     lhs
-    unfold captureNext'.go
+    unfold captureNext.go
     simp [atEnd, isSome, isNone, h₁, h₂]
 
 @[simp]
-theorem captureNext'.go_ind_found {nfa wf it matched current next matched' next'}
+theorem captureNext.go_ind_found {σ nfa wf it matched current next matched' next'}
   (atEnd : ¬it.atEnd) (isEmpty : ¬current.states.isEmpty) (isSome : matched.isSome)
-  (h : eachStepChar' nfa wf it current next = (matched', next')) :
-  captureNext'.go nfa wf it matched current next = captureNext'.go nfa wf it.next (matched' <|> matched) next' ⟨current.states.clear, current.updates⟩ := by
+  (h : eachStepChar σ nfa wf it current next = (matched', next')) :
+  captureNext.go σ nfa wf it matched current next = captureNext.go σ nfa wf it.next (matched' <|> matched) next' ⟨current.states.clear, current.updates⟩ := by
   have isNone : ¬matched.isNone := by
     cases matched <;> simp_all
   conv =>
     lhs
-    unfold captureNext'.go
+    unfold captureNext.go
     simp [atEnd, isEmpty, isSome, isNone, h]
 
 end
