correctness/RegexCorrectness/VM/Search/Compile.lean
@@ -10,13 +10,13 @@ open String (Pos Iterator)
 
 namespace Regex.VM
 
-theorem captures_of_captureNext'_some {e nfa it matched'} (eq : NFA.compile e = nfa)
-  (h : captureNext' nfa (eq ▸ NFA.compile_wf) it = matched') (v : it.Valid) (isSome' : matched'.isSome) :
+theorem captures_of_captureNext_some {e nfa it matched'} (eq : NFA.compile e = nfa)
+  (h : captureNext HistoryStrategy nfa (eq ▸ NFA.compile_wf) it = matched') (v : it.Valid) (isSome' : matched'.isSome) :
   ∃ l r span groups,
     span.toString = it.toString ∧
     e.Captures ⟨l, [], r⟩ span groups ∧
     EquivUpdate groups (matched'.get isSome') := by
-  have ⟨state, span, eqstring, hn, path⟩ := captureNext'.path_done_of_matched h v isSome'
+  have ⟨state, span, eqstring, hn, path⟩ := captureNext.path_done_of_matched h v isSome'
   have eq_zero := (NFA.done_iff_zero_compile eq state).mp hn
   have : state.val ≠ nfa.start := by
     simp [eq_zero]
