correctness/RegexCorrectness/VM/Search/Lemmas.lean
@@ -16,19 +16,19 @@ def MatchedInv (nfa : NFA) (wf : nfa.WellFormed) (it₀ : Iterator) (matched : O
       nfa[state] = .done ∧
       nfa.VMPath wf span state (matched.get isSome)
 
-theorem captureNext'.go.inv {nfa wf it₀ it matched current next matched'}
-  (h : captureNext'.go nfa wf it matched current next = matched')
+theorem captureNext.go.inv {nfa wf it₀ it matched current next matched'}
+  (h : captureNext.go HistoryStrategy nfa wf it matched current next = matched')
   (v : it.Valid) (string_eq : it.toString = it₀.toString)
   (curr_inv : current.Inv nfa wf it) (empty : next.states.isEmpty)
   (matched_inv : MatchedInv nfa wf it₀ matched) :
   MatchedInv nfa wf it₀ matched' := by
-  induction it, matched, current, next using captureNext'.go.induct' nfa wf with
+  induction it, matched, current, next using captureNext.go.induct' HistoryStrategy nfa wf with
   | not_found it matched current next atEnd => simp_all
   | found it matched current next atEnd empty' some =>
-    rw [captureNext'.go_found atEnd empty' some] at h
+    rw [captureNext.go_found atEnd empty' some] at h
     simp_all
   | ind_not_found it matched current next _ current' matched'' next' atEnd isNone h₁ h₂ ih =>
-    rw [captureNext'.go_ind_not_found atEnd isNone h₁ h₂] at h
+    rw [captureNext.go_ind_not_found atEnd isNone h₁ h₂] at h
     have curr'_inv := εClosure.inv_of_inv h₁ v curr_inv
     have next'_inv := eachStepChar.inv_of_inv h₂ atEnd empty curr'_inv
     have matched''_inv : MatchedInv nfa wf it₀ matched'' := by
@@ -46,7 +46,7 @@ theorem captureNext'.go.inv {nfa wf it₀ it matched current next matched'}
       exact ⟨state', span, eqstring, hn, path⟩
     exact ih h (v.next (it.hasNext_of_not_atEnd atEnd)) string_eq next'_inv (by simp) matched''_inv
   | ind_found it matched current next matched'' next' atEnd empty' isSome h' ih =>
-    rw [captureNext'.go_ind_found atEnd empty' isSome h'] at h
+    rw [captureNext.go_ind_found atEnd empty' isSome h'] at h
     have next'_inv := eachStepChar.inv_of_inv h' atEnd empty curr_inv
     have matched''_inv : MatchedInv nfa wf it₀ (matched'' <|> matched) := by
       cases matched'' with
@@ -71,15 +71,15 @@ theorem captureNext'.go.inv {nfa wf it₀ it matched current next matched'}
 If `captureNext'` returns `some`, the returned list corresponds to the updates of a path from
 `nfa.start` to a `.done` state.
 -/
-theorem captureNext'.path_done_of_matched {nfa wf it matched'}
-  (h : captureNext' nfa wf it = matched') (v : it.Valid) (isSome' : matched'.isSome) :
+theorem captureNext.path_done_of_matched {nfa wf it matched'}
+  (h : captureNext HistoryStrategy nfa wf it = matched') (v : it.Valid) (isSome' : matched'.isSome) :
   ∃ state span,
     span.toString = it.toString ∧
     nfa[state] = .done ∧
     nfa.VMPath wf span state (matched'.get isSome') := by
-  simp [captureNext'] at h
+  simp [captureNext] at h
 
-  set result := εClosure' nfa wf it .none ⟨.empty, Vector.mkVector nfa.nodes.size []⟩ [([], ⟨nfa.start, wf.start_lt⟩)]
+  set result := εClosure HistoryStrategy nfa wf it .none ⟨.empty, Vector.mkVector nfa.nodes.size []⟩ [([], ⟨nfa.start, wf.start_lt⟩)]
   set matched := result.1
   set current := result.2
   have h' : result = (matched, current) := rfl
@@ -92,6 +92,6 @@ theorem captureNext'.path_done_of_matched {nfa wf it matched'}
     simp [WriteUpdate, hn, hupdate] at write
     exact ⟨state, span, by simp [←eqit, Span.iterator], hn, write ▸ path⟩
 
-  exact captureNext'.go.inv h v rfl curr_inv (by simp) matched_inv isSome'
+  exact captureNext.go.inv h v rfl curr_inv (by simp) matched_inv isSome'
 
 end Regex.VM
